bedrock2/src/bedrock2Examples/roughtime.v
@@ -5,6 +5,7 @@ Require Import bedrock2.Syntax bedrock2.NotationsInConstr bedrock2.NotationsCust
 Import Syntax BinInt String List.ListNotations ZArith.
 From coqutil Require Import Word.Interface Map.Interface.
 Require Import coqutil.Byte coqutil.Z.HexNotation coqutil.Z.Lia.
+Require Import Coq.Strings.Ascii.
 
 Local Open Scope string_scope. Local Open Scope Z_scope. Local Open Scope list_scope.
 Local Coercion literal (z : Z) : Syntax.expr := Syntax.expr.literal z.
@@ -13,10 +14,19 @@ Local Definition bedrock_func : Type :=
   String.string * (list String.string * list String.string * cmd).
 Local Coercion name_of_func (f : bedrock_func) := fst f.
 
-Definition stringToHex (s : string) : Z := Ox"ffffffff".
 
-Lemma stringHexBound : forall s, 0 <= stringToHex s < 2^32.
-Proof. intros s. unfold stringToHex. cbn. blia. Qed.
+Fixpoint N_of_string (s : string) : N :=
+  match s with
+  | EmptyString => 0
+  | String a s => (N_of_ascii a) + 256 * (N_of_string s)
+  end.
+
+Definition Z_of_string (s : string) := Z.of_N (N_of_string s).
+
+Lemma stringHexBound : forall s, (length s <= 4)%nat -> 0 <= Z_of_string s < 2^32.
+Proof.
+  intros s.
+Admitted.
 
 Definition createTimestampMessage :=
   let buffer := "buffer" in
@@ -28,11 +38,11 @@ Definition createTimestampMessage :=
     store4(buffer + coq:(12), coq:(Ox"a4"));
     store4(buffer + coq:(16), coq:(Ox"13c"));
 
-    store4(buffer + coq:(20), coq:(stringToHex "SIG"));
-    store4(buffer + coq:(24), coq:(stringToHex "PATH"));
-    store4(buffer + coq:(28), coq:(stringToHex "SREP"));
-    store4(buffer + coq:(32), coq:(stringToHex "CERT"));
-    store4(buffer + coq:(36), coq:(stringToHex "INDX"));
+    store4(buffer + coq:(20), coq:(Z_of_string "SIG"));
+    store4(buffer + coq:(24), coq:(Z_of_string "PATH"));
+    store4(buffer + coq:(28), coq:(Z_of_string "SREP"));
+    store4(buffer + coq:(32), coq:(Z_of_string "CERT"));
+    store4(buffer + coq:(36), coq:(Z_of_string "INDX"));
 
     i = (coq:(64)); while (i) { i = (i - coq:(4));
       store4(buffer + coq:(100) - i, coq:(Ox"42"))
@@ -42,13 +52,42 @@ Definition createTimestampMessage :=
     store4(buffer + coq:(108), coq:(Ox"4"));
     store4(buffer + coq:(112), coq:(Ox"c"));
 
-    store4(buffer + coq:(116), coq:(stringToHex "RADI"));
-    store4(buffer + coq:(120), coq:(stringToHex "MIDP"));
-    store4(buffer + coq:(124), coq:(stringToHex "ROOT"));
+    store4(buffer + coq:(116), coq:(Z_of_string "RADI"));
+    store4(buffer + coq:(120), coq:(Z_of_string "MIDP"));
+    store4(buffer + coq:(124), coq:(Z_of_string "ROOT"));
     
-    store4(buffer + coq:(128), coq:(Ox"42424242"));
-    store(buffer + coq:(232), coq:(Ox"4242424242424242"))
-  ))).
+    store4(buffer + coq:(128), coq:(Ox"4242"));
+    store4(buffer + coq:(132), coq:(Ox"42424242"));
+    i = (coq:(64)); while (i) { i = (i - coq:(4));
+      store4(buffer + coq:(200) - i, coq:(Ox"42"))
+    };
+
+    store4(buffer + coq:(204), coq:(Ox"2"));
+    store4(buffer + coq:(208), coq:(Ox"40"));
+    store4(buffer + coq:(212), coq:(Z_of_string "SIG"));
+    store4(buffer + coq:(216), coq:(Z_of_string "DELE"));
+    i = (coq:(64)); while (i) { i = (i - coq:(4));
+      store4(buffer + coq:(280) - i, coq:(Ox"42"))
+    };
+
+    store4(buffer + coq:(284), coq:(Ox"3"));
+    store4(buffer + coq:(288), coq:(Ox"20"));
+    store4(buffer + coq:(292), coq:(Ox"28"));
+
+    store4(buffer + coq:(296), coq:(Z_of_string "PUBK"));
+    store4(buffer + coq:(300), coq:(Z_of_string "MINT"));
+    store4(buffer + coq:(304), coq:(Z_of_string "MAXT"));
+ 
+    i = (coq:(48)); while (i) { i = (i - coq:(4));
+      store4(buffer + coq:(352) - i, coq:(Ox"42"))
+    };
+
+    store4(buffer + coq:(356), coq:(Ox"43"))))).
+    
+Require Import bedrock2.ToCString.
+   Definition allProgsAsCString : string :=
+     Eval cbv in c_module [createTimestampMessage].
+   Print allProgsAsCString.
 
 Require bedrock2.WeakestPrecondition.
 Require Import bedrock2.Semantics bedrock2.FE310CSemantics.
@@ -65,18 +104,17 @@ Require Import coqutil.Tactics.rewr.
 Section WithParameters.
   Context {p : FE310CSemantics.parameters}.
 
-  Definition entry: Type := string * Semantics.word * (Semantics.word -> mem -> Prop).
-
+  Definition entry : Type := string * Semantics.word * (Semantics.word -> mem -> Prop).
+  
   Infix "*" := (sep).
   Infix "*" := (sep) : type_scope.
 
   Infix "+" := (word.add).
   Infix "+" := (word.add) : type_scope.
 
-  
   Notation array32 := (array scalar32 (word.of_Z 4)).
   
-  Definition stringToWord (s : string) := word.of_Z (stringToHex s).
+  Definition stringToWord (s : string) := word.of_Z (Z_of_string s).
 
   Definition size_field (addr: Semantics.word) (entries : list entry) : mem -> Prop :=
     scalar32 addr (word.of_Z (Z.of_nat (List.length entries))).
@@ -104,17 +142,29 @@ Section WithParameters.
   Definition repeat_dummy n := fun addr => array32 (addr: Semantics.word) (List.repeat (word.of_Z (Ox"42")) n).
 
   Definition srep_val : list entry :=
-    [("RADI", word.of_Z 0, repeat_dummy 4);
-    ("MIDP", word.of_Z 4, repeat_dummy 8);
-    ("ROOT", word.of_Z 12, repeat_dummy 64)
+    [("RADI", word.of_Z 0, fun _ => (emp True));
+    ("MIDP", word.of_Z 4,  fun _ => (emp True));
+    ("ROOT", word.of_Z 12,  fun _ => (emp True))
+    ].
+
+  Definition dele_val : list entry :=
+    [("MINT", word.of_Z 0, fun _ => (emp True));
+    ("MAXT", word.of_Z 32,  fun _ => (emp True));
+    ("PUBK", word.of_Z 40,  fun _ => (emp True))
+    ].
+
+  Definition cert_val : list entry :=
+    [("SIG", word.of_Z 0, fun _ => (emp True));
+    ("DELE", word.of_Z 64, fun addr => message_ok addr dele_val)
     ].
   
+  
   Definition message_val : list entry :=
-    [("SIG", word.of_Z 0, repeat_dummy 64);
-    ("PATH", word.of_Z 64, repeat_dummy 64);
+    [("SIG", word.of_Z 0, fun _ => (emp True));
+    ("PATH", word.of_Z 64, fun _ => (emp True));
     ("SREP", word.of_Z 64, fun addr => message_ok addr srep_val);
-    ("CERT", word.of_Z 164, repeat_dummy 64);
-    ("INDX", word.of_Z 316, repeat_dummy 64)
+    ("CERT", word.of_Z 164, fun addr => message_ok addr cert_val);
+    ("INDX", word.of_Z 316, fun _ => (emp True))
     ].
     
 
@@ -141,23 +191,30 @@ Section WithParameters.
        match goal with
        | |- context [?a + ?b] => progress (ring_simplify (a + b))
        | |- context [word.sub ?a ?b] => progress (ring_simplify (word.sub a b))
-       | |- context [ (word.unsigned (word.of_Z ?z))] => rewrite (word.unsigned_of_Z z); replace (word.wrap z) with z by (cbn; blia)
-       | |- context [word.of_Z (word.unsigned ?z)] => rewrite (word.of_Z_unsigned z)
        end.
+
+   Ltac word_Z_unsigned :=
+     match goal with
+     | |- context [ (word.unsigned (word.of_Z ?z))] => rewrite (word.unsigned_of_Z z); change (word.wrap z) with z
+     | |- context [word.of_Z (word.unsigned ?z)] => rewrite (word.of_Z_unsigned z)
+     end.
 
    Ltac word_simplify_in H :=
        match type of H with 
        | context [?a + ?b] => progress (ring_simplify (a + b) in H)
        | context [word.sub ?a ?b] => progress (ring_simplify (word.sub a b) in H)
-       | context [word.unsigned (word.of_Z ?z)] => rewrite (word.unsigned_of_Z z) in H; replace (word.wrap z) with z in H by (cbn; blia)
-       | context [word.of_Z (word.unsigned ?z)] => rewrite (word.of_Z_unsigned z) in H
        end.
+   Ltac word_Z_unsigned_in H:=
+     match type of H with
+     | context [word.unsigned (word.of_Z ?z)] => rewrite (word.unsigned_of_Z z) in H; change (word.wrap z) with z in H
+     | context [word.of_Z (word.unsigned ?z)] => rewrite (word.of_Z_unsigned z) in H
+     end.
 
    Ltac word_unwrap t :=
-     unfold word.wrap; rewrite Zmod_small; [| assert (0 <= t < 2^32) by blia; assumption].
+     unfold word.wrap; rewrite (Zmod_small t); [| assert (0 <= t < 2^width) by blia; assumption].
 
    Ltac word_unwrap_in t H :=
-     unfold word.wrap in H; rewrite Zmod_small in H; [| assert (0 <= t < 2^32) by blia; assumption].
+     unfold word.wrap in H; rewrite (Zmod_small t) in H; [| assert (0 <= t < 2^width) by blia; assumption].
 
    Definition todo : False. Admitted.
    
@@ -166,16 +223,210 @@ Section WithParameters.
      repeat straightline.
      do 10 (destruct buf; [inversion H0|]).
      inversion H0; clear H0.
+     unfold Array.array in H.
+     unfold WeakestPrecondition.store.
+     
+     straightline.
+     
      cbn[Array.array] in H.
-     do 9 (word_simplify_in H).
+     (* Make a helper lemma that says what happens if I set a value inside an array 
+        straightline can invoke such lemma:
+
+
+  Lemma store_four_of_sep addr (oldvalue : word32) (value : word) R m (post:_->Prop)
+    (Hsep : sep (scalar32 addr oldvalue) R m)
+    (Hpost : forall m, sep (scalar32 addr (word.of_Z (word.unsigned value))) R m -> post m)
+    : exists m1, Memory.store Syntax.access_size.four m addr value = Some m1 /\ post m1.
+
+(* Ideally I would be able to compute n and not have to specify it *)
+Lemma store_four_of_sep addr (oldvalues : list word32) (value : word) R m (post:_->Prop) (_ : addr' = addr + size * n) (_ : n < length oldvalues)
+    (Hsep : sep (array32 addr oldvalues) R m)
+    (Hpost : forall m, sep (array32 addr oldvalues[n |-> value]) R m -> post m)
+    : exists m1, Memory.store Syntax.access_size.four m (addr') value = Some m1 /\ post m1.
+
+Conclusion: Weakestprecondition.store access_size.four m p_addr v post
+
+
+      *)
+
+     
+     ring_simplify (p_addr + lit 4 + lit 4 + lit 4 + lit 4 + lit 4 + lit 4 + lit 4 +
+                    lit 4 + lit 4 + lit 4).
+     (word_simplify_in H).
+     Eval cbn in (lit (4 + 4)).
+     (word_simplify_in H).
+     (word_simplify_in H).
+     (word_simplify_in H).
+     (word_simplify_in H).
+     (word_simplify_in H).
+     (word_simplify_in H).
+     
+     
      repeat straightline.
      subst_words.
      clear H9 H8 H7 H6 H5 H4 H3 H1 H0 H.
-     repeat word_simplify_in H10.
+     repeat word_Z_unsigned_in H10.
+       
+     
+     refine ((TailRecursion.tailrec (HList.polymorphic_list.cons _ HList.polymorphic_list.nil) ("i"::"buffer"::nil)%list%string (fun V R T M I BUFFER => PrimitivePair.pair.mk (exists i, V = 64 - 4 * (Z.of_nat i) /\ V = word.unsigned I /\ BUFFER = p_addr /\ (array32 (p_addr + (lit 40)) (List.repeat (word.of_Z (Ox"42")) i) * array32 (p_addr + (lit (104 - V))) (List.skipn i buf) * array32 p_addr (List.map word.of_Z [5; 64; 64; 164; 316; Z_of_string "SIG"; Z_of_string "PATH"; Z_of_string "SREP"; Z_of_string "CERT"; Z_of_string "INDX"]) * R) M) (fun t m i buff => t = T /\ buff = p_addr /\ (array32 p_addr (List.map word.of_Z ([5; 64; 64; 164; 316; Z_of_string "SIG"; Z_of_string "PATH"; Z_of_string "SREP"; Z_of_string "CERT"; Z_of_string "INDX"] ++ (List.repeat (Ox"42") 16))) * array32 (p_addr + (lit (104))) (List.skipn 16%nat buf) * R) m))) _ _ _ _ _ _ _);
+      cbn [reconstruct map.putmany_of_list HList.tuple.to_list
+           HList.hlist.foralls HList.tuple.foralls
+           HList.hlist.existss HList.tuple.existss
+           HList.hlist.apply  HList.tuple.apply
+           HList.hlist
+
+           List.repeat Datatypes.length
+           HList.polymorphic_list.repeat HList.polymorphic_list.length
+           PrimitivePair.pair._1 PrimitivePair.pair._2] in *.
+
+     { repeat straightline. }
+     { eapply (Z.lt_wf 0). }
+     { exists 0%nat.
+       split; auto.
+       split; try word_Z_unsigned; try split; try split; try blia; auto.
+       word_simplify.
+       cbn [List.repeat Array.array List.skipn List.map].
+       change (Z_of_string "SIG") with 4671827.
+       change (Z_of_string "PATH") with 1213481296.
+       change (Z_of_string "SREP") with 1346720339.
+       change (Z_of_string "CERT") with 1414677827.
+       change (Z_of_string "INDX") with 1480871497.
+       repeat word_simplify.
+       ecancel_assumption. }
+     { repeat straightline.
+       2: {
+         split; try split; auto.
+         replace x2 with 16%nat in H3, H by blia.
+         simpl in H.
+         rewrite H in H3.
+         change (104-0) with 104 in H3.
+         rewrite map_app.
+         array_app_cons_sep.
+         cbn [List.length List.map] in *. (*TODO: this can be improved*)
+         word_simplify.
+         unfold repeat in H3.
+         ecancel_assumption. }
+         
+       subst_words.
+       word_simplify.
+       subst v.
+       repeat word_simplify_in H3.
+       word_Z_unsigned_in H3.
+       pose proof (word.unsigned_range x0).
+       assert (List.length (List.skipn x2 buf) <> 0%nat) by (rewrite List.skipn_length; blia).
+       destruct (List.skipn x2 buf) eqn:H17; try contradiction.
+       array_app_cons_sep.
+       repeat straightline.
+       subst_words.
+       eexists; eexists; split.
+       { exists (1 + x2)%nat.
+         replace (64 - 4 * Z.of_nat (1 + x2)) with (60 - 4 * Z.of_nat x2) by blia.
+         split; auto.
+         split; try split; try split; auto.
+         { rewrite word.unsigned_sub.
+           word_Z_unsigned.
+           word_unwrap (word.unsigned x0 - 4).
+           blia.
+         }
+         { pose proof (f_equal word.of_Z H).
+           word_Z_unsigned_in H7.
+           rewrite H7 in H6.
+           change (1 + x2)%nat with (S x2)%nat.
+           cbn [List.repeat].
+           rewrite repeat_cons.
+           array_app_cons_sep.
+           rewrite repeat_length, <- List.tl_skipn, H17.
+           cbn[List.tl].
+           (*Set Ltac Profiling.*)
+           repeat word_simplify.
+           (*Show Ltac Profile.*)
+           repeat word_simplify_in H6.
+           word_Z_unsigned_in H6.
+           change (66) with (Ox "42") in H6.
+           ecancel_assumption.
+         }
+       }
+       eexists; eexists; try blia; destruct H7; auto.
+     }
+     repeat straightline.
+
+     clear H10.
+     pose proof (firstn_skipn 16%nat buf).
+     remember (List.skipn 16%nat buf) as buf'.
+     pose proof (f_equal (@List.length _) H).
+     rewrite H2, app_length, firstn_length in H0.
+     assert (List.length buf' = 998)%nat by blia.
+     clear H; clear H0; clear Heqbuf'; clear H2.
+     do 9 (destruct buf' ; [inversion H3|]).
+     inversion H3; clear H3.
+     cbn[Array.array] in H1.
+     repeat (word_simplify_in H1).
+     repeat straightline.
+     subst_words.
+     clear H7 H6 H5 H4 H3 H2 H1 H.
+     repeat word_Z_unsigned_in H8.
+     repeat straightline.
+
+     
+
+     
+     
+     refine ((TailRecursion.tailrec (HList.polymorphic_list.cons _ HList.polymorphic_list.nil) ("i"::"buffer"::nil)%list%string (fun V R T M I BUFFER => PrimitivePair.pair.mk (exists i, V = 64 - 4 * (Z.of_nat i) /\ V = word.unsigned I /\ (i < 16)%nat /\ BUFFER = p_addr /\ (array32 (p_addr + (lit 40)) (List.repeat (word.of_Z (Ox"42")) i) * array32 (p_addr + (lit (104 - V))) (List.skipn i buf) * array32 p_addr (List.map word.of_Z [5; 64; 64; 164; 316; Z_of_string "SIG"; Z_of_string "PATH"; Z_of_string "SREP"; Z_of_string "CERT"; Z_of_string "INDX"]) * R) M) (fun t m i buf => t = T))) _ _ _ _ _ _ _);
+      cbn [reconstruct map.putmany_of_list HList.tuple.to_list
+           HList.hlist.foralls HList.tuple.foralls
+           HList.hlist.existss HList.tuple.existss
+           HList.hlist.apply  HList.tuple.apply
+           HList.hlist
+
+           List.repeat Datatypes.length
+           HList.polymorphic_list.repeat HList.polymorphic_list.length
+           PrimitivePair.pair._1 PrimitivePair.pair._2] in *.
+
+     { repeat straightline. }
+     { eapply (Z.lt_wf 0). }
+     { exists 0%nat.
+       split; auto.
+       split; try word_Z_unsigned; try split; try split; try blia; auto.
+       word_simplify.
+       cbn [List.repeat Array.array List.skipn List.map].
+       change (Z_of_string "SIG") with 4671827.
+       change (Z_of_string "PATH") with 1213481296.
+       change (Z_of_string "SREP") with 1346720339.
+       change (Z_of_string "CERT") with 1414677827.
+       change (Z_of_string "INDX") with 1480871497.
+       repeat word_simplify.
+       ecancel_assumption. }
+     { repeat straightline.
+       subst_words.
+       word_simplify.
+       subst v.
+       repeat word_simplify_in H4.
+       word_Z_unsigned_in H4.
+       assert (List.length (List.skipn x2 buf) <> 0%nat) by (rewrite List.skipn_length; blia).
+       destruct (List.skipn x2 buf) eqn:H17; try contradiction.
+       array_app_cons_sep.
+       repeat straightline.
+       subst_words.
+       eexists; eexists; split.
+       { exists (1 + x2)%nat.
+         replace (64 - 4 * Z.of_nat (1 + x2)) with (60 - 4 * Z.of_nat x2) by blia.
+         split; auto.
+         split; try split; try split; auto.
+         { rewrite word.unsigned_sub.
+           word_Z_unsigned.
+           word_unwrap (word.unsigned x0 - 4).
+           blia.
+         }
+         { rewrite word.unsigned_sub in H5.
+           word_Z_unsigned_in H5.
+           word_unwrap_in (word.unsigned x - 4) H5.
+           blia.
+         }
+     
      
      refine ((TailRecursion.atleastonce ["i"; "buffer"] (fun V T M I BUFFER =>
        exists i, V = 64 - 4 * (Z.of_nat i) /\
-       V = word.unsigned I /\ (i < 16)%nat /\ BUFFER = p_addr /\ (array32 (p_addr + (lit 40)) (List.repeat (word.of_Z (Ox"42")) i) * array32 (p_addr + (lit (104 - V))) (List.skipn i buf) * array32 p_addr (List.map word.of_Z [5; 64; 64; 164; 316; 4294967295; 4294967295; 4294967295; 4294967295; 4294967295]) * R) M
+       V = word.unsigned I /\ (i < 16)%nat /\ BUFFER = p_addr /\ (array32 (p_addr + (lit 40)) (List.repeat (word.of_Z (Ox"42")) i) * array32 (p_addr + (lit (104 - V))) (List.skipn i buf) * array32 p_addr (List.map word.of_Z [5; 64; 64; 164; 316; Z_of_string "SIG"; Z_of_string "PATH"; Z_of_string "SREP"; Z_of_string "CERT"; Z_of_string "INDX"]) * R) M
        )) _ _ _ _ _ _ _);
       cbn [reconstruct map.putmany_of_list HList.tuple.to_list
            HList.hlist.foralls HList.tuple.foralls
@@ -189,14 +440,138 @@ Section WithParameters.
 
      { repeat straightline. }
      { eapply (Z.lt_wf 0). }
-     { repeat straightline.
-       shelve. }
+     { eexists; split; repeat straightline.
+       word_Z_unsigned_in H.
+       blia. }
      { exists 0%nat.
        split; auto.
-       split; word_simplify; try split; try split; try blia; auto.
+       split; try word_Z_unsigned; try split; try split; try blia; auto.
        word_simplify.
        cbn [List.repeat Array.array List.skipn List.map].
+       change (Z_of_string "SIG") with 4671827.
+       change (Z_of_string "PATH") with 1213481296.
+       change (Z_of_string "SREP") with 1346720339.
+       change (Z_of_string "CERT") with 1414677827.
+       change (Z_of_string "INDX") with 1480871497.
        repeat word_simplify.
+       ecancel_assumption. }
+     repeat straightline.
+     subst_words.
+     subst v.
+     word_simplify.
+     repeat (word_simplify_in H4).
+     word_Z_unsigned_in H4.
+     assert (List.length (List.skipn x1 buf) <> 0%nat) by (rewrite List.skipn_length; blia).
+     destruct (List.skipn x1 buf) eqn:H17; try contradiction.
+     array_app_cons_sep.
+     repeat straightline.
+     { subst_words.
+       eexists; auto.
+       split.
+       - exists (1 + x1)%nat.
+         replace (64 - 4 * Z.of_nat (1 + x1)) with (60 - 4 * Z.of_nat x1) by blia.
+         split; auto.
+         split; try split; try split; auto.
+         { rewrite word.unsigned_sub.
+           word_Z_unsigned.
+           word_unwrap (word.unsigned x - 4).
+           blia.
+         }
+         { rewrite word.unsigned_sub in H5.
+           word_Z_unsigned_in H5.
+           word_unwrap_in (word.unsigned x - 4) H5.
+           blia.
+         }
+         pose proof (f_equal word.of_Z H).
+         word_Z_unsigned_in H6.
+         rewrite H6 in H3.
+         change (1 + x1)%nat with (S x1)%nat.
+         cbn [List.repeat].
+         rewrite repeat_cons.
+         array_app_cons_sep.
+         rewrite repeat_length, <- List.tl_skipn, H17.
+         cbn[List.tl].
+         (*Set Ltac Profiling.*)
+         repeat word_simplify.
+         (*Show Ltac Profile.*)
+         repeat word_simplify_in H3.
+         word_Z_unsigned_in H3.
+         change (66) with (Ox "42") in H3.
+         ecancel_assumption.
+       - blia.
+     }
+     clear H4.
+     subst br.
+     rewrite word.unsigned_sub in H5.
+     word_Z_unsigned_in H5.
+     word_unwrap_in (word.unsigned x - 4) H5.
+     assert (word.unsigned x = 4) by blia.
+     pose proof (f_equal word.of_Z H4).
+     word_Z_unsigned_in H6.
+     rewrite H6 in H3, H.
+     repeat word_simplify_in H3.
+     word_Z_unsigned_in H.
+     assert (x1 = 15)%nat by blia.
+     clear H4; clear H6; clear H5.
+     rewrite H7 in *; clear H7.
+     clear H; clear H1.
+     pose proof (f_equal (@List.length _) (firstn_skipn 15 buf)).
+     rewrite H2, app_length, firstn_length, H17, List.length_cons, H2 in H.
+     assert (List.length l0 = 998)%nat by blia.
+     clear H; clear H0; clear H17.
+     
+     do 9 (destruct l0; [inversion H1|]).
+     inversion H1; clear H1.
+     cbn[Array.array] in H3.
+     repeat (word_simplify_in H3).
+     repeat straightline.
+     subst_words.
+     clear H10 H8 H7 H6 H5 H4 H3 H1 H.
+     repeat word_Z_unsigned_in H9.
+     repeat straightline.
+
+     remember (map word.of_Z
+                   [5; 64; 64; 164; 316; Z_of_string "SIG";
+                    Z_of_string "PATH"; Z_of_string "SREP"; 
+                    Z_of_string "CERT"; Z_of_string "INDX"]) as buf1.
+     
+
+     refine ((TailRecursion.atleastonce ["i"; "buffer"] (fun V T M I BUFFER =>
+       exists i, V = 64 - 4 * (Z.of_nat i) /\
+       V = word.unsigned I /\ (i < 16)%nat /\ BUFFER = p_addr /\ (array32 (p_addr + (lit 140)) (List.repeat (word.of_Z (Ox"42")) i) * array32 (p_addr + (lit (204 - V))) (List.skipn i buf) * array32 p_addr (List.map word.of_Z ([5; 64; 64; 164; 316; Z_of_string "SIG"; Z_of_string "PATH"; Z_of_string "SREP"; Z_of_string "CERT"; Z_of_string "INDX"] ++ (List.repeat ((Ox"42")) 16) ++ [3; 4; 12; Z_of_string "RADI"; Z_of_string "MIDP"; Z_of_string "ROOT"; Ox"4242"; Ox"42424242"])) * R) M
+       )) _ _ _ _ _ _ _);
+      cbn [reconstruct map.putmany_of_list HList.tuple.to_list
+           HList.hlist.foralls HList.tuple.foralls
+           HList.hlist.existss HList.tuple.existss
+           HList.hlist.apply  HList.tuple.apply
+           HList.hlist
+
+           List.repeat Datatypes.length
+           HList.polymorphic_list.repeat HList.polymorphic_list.length
+           PrimitivePair.pair._1 PrimitivePair.pair._2] in *.
+
+     { repeat straightline. }
+     { eapply (Z.lt_wf 0). }
+     { eexists; split; repeat straightline.
+       word_Z_unsigned_in H.
+       blia. }
+     { exists 0%nat.
+       split; auto.
+       split; try word_Z_unsigned; try split; try split; try blia; auto.
+       word_simplify.
+       rewrite map_app, map_app.
+       cbn[List.map].
+       
+       
+       cbn [List.map List.repeat List.app Array.array List.skipn].
+       
+       change (Z_of_string "RADI") with 1229209938.
+       change (Z_of_string "MIDP") with 1346652493.
+       change (Z_of_string "ROOT") with 1414483794.
+
+       
+       
+       do 20 word_simplify.
        ecancel_assumption. }
      repeat straightline.
      subst_words.
@@ -233,36 +608,23 @@ Section WithParameters.
          array_app_cons_sep.
          rewrite repeat_length, <- List.tl_skipn, H17.
          cbn[List.tl].
-         Set Ltac Profiling.
+         (*Set Ltac Profiling.*)
          repeat word_simplify.
-         Show Ltac Profile.
+         (*Show Ltac Profile.*)
          repeat word_simplify_in H3.
          change (66) with (Ox "42") in H3.
          ecancel_assumption.
        - blia.
      }
-     clear H4.
-     subst br.
-     rewrite word.unsigned_sub in H5.
-     word_simplify_in H5.
-     word_unwrap_in (word.unsigned x - 4) H5.
-     assert (word.unsigned x = 4) by blia.
-     pose proof (f_equal word.of_Z H4).
-     word_simplify_in H6.
-     rewrite H6 in H3, H.
-     repeat word_simplify_in H3.
-     word_simplify_in H.
-     assert (x1 = 15)%nat by blia.
-     clear H4; clear H6; clear H5.
-     rewrite H7 in *; clear H7.
-     clear H; clear H1.
-     pose proof (f_equal (@List.length _) (firstn_skipn 15 buf)).
-     rewrite H2, app_length, firstn_length, H17, List.length_cons, H2 in H.
-     assert (List.length l0 = 998)%nat by blia.
-     exfalso.
-     exact todo.
+     
+
+     destruct todo.
+
+     
+   Qed.
+
+
    
-                                 
    
    Lemma createTimestampMessage_ok : program_logic_goal_for_function! createTimestampMessage.
    Proof.
